@prefix rdfs: <http://www.w3.org/2000/01/rdf-schema#>.
@prefix owl: <http://www.w3.org/2002/07/owl#>.
@prefix xsd: <http://www.w3.org/2001/XMLSchema#>.
@prefix skos: <http://www.w3.org/2004/02/skos/core#>.
@prefix dct: <http://purl.org/dc/terms/>.
@prefix foaf: <http://xmlns.com/foaf/0.1/>.
@prefix cidoc: <http://www.cidoc-crm.org/cidoc-crm/>.
@prefix nie-ine-event: <http://e-editiones.ch/ontology/event#>.
@prefix nie-ine-human: <http://e-editiones.ch/ontology/human#>.


@base <https://github.com/stazh/sw-ehedaten/tree/main/ontology/marriage>.
@prefix marriage: <https://github.com/stazh/sw-ehedaten/tree/main/ontology/marriage#>.

<https://github.com/stazh/sw-ehedaten/tree/main/ontology/marriage>
	a owl:Ontology;
	dct:license <http://creativecommons.org/licenses/by/3.0/>;
	dct:title "An ontology about marriage"@en;
	dct:description """Formal description of a marriage, general subclasses, related classes and properties."""@en;
	dct:creator "Rebekka Pl체ss, research assistant and software developer, States Archive canton of Z체rich"@en;
	dct:publisher "States Archive canton of Z체rich"@en;
	owl:versionInfo "2021-11-26"^^xsd:date.

#
# CLASSES
#
marriage:Marriage
	rdfs:isDefinedBy <https://github.com/stazh/sw-ehedaten/tree/main/ontology/marriage#>;
	a rdfs:Class;
	rdfs:label "marriage"@en, "Heirat"@de;
	rdfs:comment """Marriage as the event of the union of two people."""@en;
	rdfs:subClassOf nie-ine-event:Event.

marriage:ParishBook
	rdfs:isDefinedBy <https://github.com/stazh/sw-ehedaten/tree/main/ontology/marriage#>;
	a rdfs:Class;
	rdfs:label "parish book"@en, "Pfarrbuch"@de;
	rdfs:comment """The book in which a marriage is registered resp. the marriage entry is written."""@en.

marriage:MarriageEntry
	rdfs:isDefinedBy <https://github.com/stazh/sw-ehedaten/tree/main/ontology/marriage#>;
	a rdfs:Class;
	rdfs:label "marriage entry"@en, "Eheeintrag"@de;
	rdfs:comment """Marriage entry as a note by the parish priest in a parish book stating that two persons were married on a certain day."""@en.

marriage:Bride
	rdfs:isDefinedBy <https://github.com/stazh/sw-ehedaten/tree/main/ontology/marriage#>;
	a rdfs:Class;
	rdfs:label "bride"@en, "Braut"@de;
	rdfs:comment """Role of a woman marrying."""@en;
	rdfs:subClassOf nie-ine-human:PersonRole.

marriage:Bridegroom
	rdfs:isDefinedBy <https://github.com/stazh/sw-ehedaten/tree/main/ontology/marriage#>;
	a rdfs:Class;
	rdfs:label "bridegroom"@en, "Br채utigam"@de;
	rdfs:comment """Role of a man marrying."""@en;
	rdfs:subClassOf nie-ine-human:PersonRole.


#
# PROPERTIES
#

marriage:marriageEntryIsInParishBook
	rdfs:isDefinedBy <https://github.com/stazh/sw-ehedaten/tree/main/ontology/marriage#>;
	a owl:ObjectProperty;
	rdfs:label "marriage entry is in parish book"@en, "Eheeintrag befindet sich in Pfarrbuch"@de;
	rdfs:comment """Relating a marriage entry to its parish book in which it is written."""@en;
	rdfs:domain marriage:Wedding;
	rdfs:range marriage:Parish.


