@prefix rdfs: <http://www.w3.org/2000/01/rdf-schema#> .
@prefix owl: <http://www.w3.org/2002/07/owl#> .
@prefix xsd: <http://www.w3.org/2001/XMLSchema#> .
@prefix skos: <http://www.w3.org/2004/02/skos/core#> .
@prefix dct: <http://purl.org/dc/terms/> .
@prefix rico: <https://www.ica.org/standards/RiC/ontology#> .
@prefix information-carrier: <https://e-editiones.ch/ontology/information-carrier#> .
@prefix organization: <https://e-editiones.ch/ontology/organization#> .
@prefix document: <https://e-editiones.ch/ontology/document#> .
@prefix agent: <https://e-editiones.ch/ontology/agent#> .
@prefix electronic-information: <https://e-editiones.ch/ontology/electronic-information#> .

@base <https://github.com/stazh/sw-ehedaten/tree/main/ontology/archiving.> .
@prefix archiving: <https://github.com/stazh/sw-ehedaten/tree/main/ontology/archiving#> .

<https://github.com/stazh/sw-ehedaten/tree/main/ontology/archiving>
	a owl:Ontology;
	dct:license <http://creativecommons.org/licenses/by/3.0/>;
	dct:title "An ontology about archiving"@en;
	dct:description """Formal description of a record, general subclasses, related classes and properties."""@en;
	dct:creator "Rebekka Plüss, research assistant and software developer, States Archive canton of Zürich"@en;
	dct:contributor "Hans Cools, MD, knowledge engineer, ontologist, software developer, University of Basel, Switzerland"@en;
	dct:publisher "States Archive canton of Zürich"@en;
	owl:versionInfo "2021-10-17"^^xsd:date.




#
# CLASSES
#
archiving:Archive
	rdfs:isDefinedBy <https://github.com/stazh/sw-ehedaten/tree/main/ontology/archiving#>;
	a rdfs:Class;
	rdfs:label "archive"@en, "Archiv"@de;
	rdfs:comment """Organization having a role of systematic collection, preservation, care and making accessible documents, objects etc. which hold information of the past. There are state archives which document the activities of the administration of the state, or there are archives that collect documents on specific topics - f.e. Social Archive or Women's Archive."""@en;
	rdfs:subClassOf organization:Archive.

archiving:Agent
	rdfs:isDefinedBy <https://github.com/stazh/sw-ehedaten/tree/main/ontology/archiving#>;
	a rdfs:Class;
	rdfs:label "agent"@en, "Akteur"@de;
	rdfs:comment """Something, someone, ... performing in an action."""@en;
	rdfs:subClassOf agent:Agent, rico:Agent.

archiving:Record
	rdfs:isDefinedBy <https://github.com/stazh/sw-ehedaten/tree/main/ontology/archiving#>;
	a rdfs:Class;
	rdfs:label "record"@en, "Archivverzeichniseinheit"@de;
	rdfs:comment """A record as an entry in an Archive Information System with metadata, which describe one or more manifestation of the record. A record is abstract."""@en;
	rdfs:subClassOf rico:Record.

archiving:RecordPart
	rdfs:isDefinedBy <https://github.com/stazh/sw-ehedaten/tree/main/ontology/archiving#>;
	a rdfs:Class;
	rdfs:label "record part"@en, "Teil einer Archivverzeichniseinheit"@de;
	rdfs:comment """A record part as an entry in an Archive Information System with metadata, which describe one or more manifestation of the record part."""@en;
	rdfs:subClassOf rico:RecordPart.

archiving:Title
	rdfs:isDefinedBy <https://github.com/stazh/sw-ehedaten/tree/main/ontology/archiving#>;
	a rdfs:Class;
	rdfs:label "title"@en, "Titel"@de;
	rdfs:comment """The title of the record or the record part."""@en;
	rdfs:subClassOf rico:Tilte.


archiving:Manifestation
	rdfs:isDefinedBy <https://github.com/stazh/sw-ehedaten/tree/main/ontology/archiving#>;
	a rdfs:Class;
	rdfs:label "manifestation"@en, "Ausprägung"@de;
	rdfs:comment """Carrier of information created by an agent with role provencance. The physical archived thing to which the record or the record part refers. A record or record part can refer to no manifestation, because it is lost or a record or record part can refer to more than one manifestation (f.e. if there exists a digital representation)."""@en;
	rdfs:subClassOf rico:Instantiation, information-carrier:Carrier.

archiving:Volume
	rdfs:isDefinedBy <https://github.com/stazh/sw-ehedaten/tree/main/ontology/archiving#>;
	a rdfs:Class;
	rdfs:label "volume"@en, "Band"@de;
	rdfs:comment """Volume as type of the carrier resp. the archival material type. It is also a special book: One book of a serie of books. One serie is a set of books which are mostly created for the same purpose by the same agent."""@en;
	rdfs:subClassOf archiving:Manifestation, information-carrier:Volume.

archiving:AdditionalContent
	rdfs:isDefinedBy <https://github.com/stazh/sw-ehedaten/tree/main/ontology/archiving#>;
	a rdfs:Class;
	rdfs:label "additional content"@en, "Zusatzinformation"@de;
	rdfs:comment """Some further information about a record or record part. Can be of any kind."""@en;
	rdfs:subClassOf rico:scopeAndContent.


archiving:Identifier
	rdfs:isDefinedBy <https://github.com/stazh/sw-ehedaten/tree/main/ontology/archiving#>;
	a rdfs:Class;
	rdfs:label "identifier"@en, "Identifikator"@de;
	rdfs:comment """The identifying mark with which a record or an record part or manifestation of it can be clearly identified and referenced. In the context of an archive information system, this is usually the signature."""@en;
	rdfs:subClassOf rico:Identifier.

archiving:DateOfOrigin
	rdfs:isDefinedBy <https://github.com/stazh/sw-ehedaten/tree/main/ontology/archiving#>;
	a rdfs:Class;
	rdfs:label "date of origin"@en, "Entstehungszeitraum"@de;
	rdfs:comment """The date when the archived thing was originally created."""@en;
	rdfs:subClassOf rico:Date.

archiving:Webpage
	rdfs:isDefinedBy <https://github.com/stazh/sw-ehedaten/tree/main/ontology/archiving#>;
	a rdfs:Class;
	rdfs:label "webpage"@en, "Webseite"@de;
	rdfs:comment """Webpage of the record or record part in an archive information system."""@en;
	rdfs:subClassOf electronic-information:Webpage.

archiving:RecordPartReference
	rdfs:isDefinedBy <https://github.com/stazh/sw-ehedaten/tree/main/ontology/archiving#>;
	a rdfs:Class;
	rdfs:label "record part reference"@en, "Archivverzeichniseinheitteil-Referenz"@de;
	rdfs:comment """A reference to a part of the manifestation of a record. This reference is described in the record part of a record. F.e. a record part has as manifestation a textline in a volume. And this volume is the manifestation of the record, of which the record part is part of. So in this example the record part reference is an information in the record part, which says, on which page of the volume the textline can be found."""@en;
	rdfs:subClassOf document:ContentStructureReference.


#
# PROPERTIES
#

#TODO: RecordPartHasDate

archiving:recordHasRecordPart
	rdfs:isDefinedBy <https://github.com/stazh/sw-ehedaten/tree/main/ontology/archiving#>;
	a owl:ObjectProperty;
	rdfs:label "record has record part"@en, "Archivverzeichniseinheit hat Archivverzeichniseinheitteil";
	rdfs:comment """Relating a record part to the record of which it is part of."""@en;
	rdfs:domain archiving:Record;
	rdfs:range archiving:RecordPart;
	rdfs:subPropertyOf rico:hasOrHadPart.

archiving:recordHasRecordPart
	rdfs:isDefinedBy <https://github.com/stazh/sw-ehedaten/tree/main/ontology/archiving#>;
	a owl:ObjectProperty;
	rdfs:label "record has record part"@en, "Archivverzeichniseinheit hat Archivverzeichniseinheitteil";
	rdfs:comment """Relating a record part to the record of which it is part of."""@en;
	rdfs:domain archiving:Record;
	rdfs:range archiving:RecordPart;
	rdfs:subPropertyOf rico:hasOrHadPart.

archiving:recordHasManifestation
	rdfs:isDefinedBy <https://github.com/stazh/sw-ehedaten/tree/main/ontology/archiving#>;
	a owl:ObjectProperty;
	rdfs:label "record has manifestation"@en, "Archivverzeichniseinheit hat Ausprägung";
	rdfs:comment """Relating a record to its manifestation."""@en;
	rdfs:domain archiving:Record;
	rdfs:range archiving:Manifestation;
	rdfs:subPropertyOf rico:hasInstantiation.

archiving:recordPartHasManifestation
	rdfs:isDefinedBy <https://github.com/stazh/sw-ehedaten/tree/main/ontology/archiving#>;
	a owl:ObjectProperty;
	rdfs:label "record part has manifestation"@en, "Archivverzeichniseinheitteil hat Ausprägung";
	rdfs:comment """Relating a record part to its manifestation."""@en;
	rdfs:domain archiving:RecordPart;
	rdfs:range archiving:Manifestation;
	rdfs:subPropertyOf rico:hasInstantiation.

archiving:recordHasTitle
	rdfs:isDefinedBy <https://github.com/stazh/sw-ehedaten/tree/main/ontology/archiving#>;
	a rdfs:Class;
	rdfs:label "record has title"@en, "Archivverzeichniseinheit hat Titel"@de;
	rdfs:comment """Relating a title to a record."""@en;
	rdfs:domain archiving:Record;
	rdfs:range archiving:Title;
	rdfs:subPropertyOf rico:hasOrHadTitle.

archiving:recordPartHasTitle
	rdfs:isDefinedBy <https://github.com/stazh/sw-ehedaten/tree/main/ontology/archiving#>;
	a rdfs:Class;
	rdfs:label "record part has title"@en, "Archivverzeichniseinheitteil hat Titel"@de;
	rdfs:comment """Relating a title to a record part."""@en;
	rdfs:domain archiving:RecordPart;
	rdfs:range archiving:Title;
	rdfs:subPropertyOf rico:hasOrHadTitle. 

archiving:titleHasLiteral
	rdfs:isDefinedBy <https://github.com/stazh/sw-ehedaten/tree/main/ontology/archiving#>;
	a owl:ObjectProperty;
	rdfs:label "title has literal"@en, "Titel hat Literal";
	rdfs:comment """Relating a title to its literal."""@en;
	rdfs:domain archiving:Title;
	rdfs:range rdfs:Literal.

archiving:recordHasDateOfOrigin
	rdfs:isDefinedBy <https://github.com/stazh/sw-ehedaten/tree/main/ontology/archiving#>;
	a rdfs:Class;
	rdfs:label "record has date of origin"@en, "Archivverzeichniseinheit hat Entstehungszeitraum"@de;
	rdfs:comment """Relating a date of origin to a record."""@en;
	rdfs:domain archiving:Record;
	rdfs:range archiving:DateOfOrigin.

archiving:recordPartHasDateOfOrigin
	rdfs:isDefinedBy <https://github.com/stazh/sw-ehedaten/tree/main/ontology/archiving#>;
	a rdfs:Class;
	rdfs:label "record part has dat of origin"@en, "Archivverzeichniseinheitteil hat Entstehungszeitraum"@de;
	rdfs:comment """Relating a date of origin to a record part."""@en;
	rdfs:domain archiving:RecordPart;
	rdfs:range archiving:DateOfOrigin.

archiving:dateOfOriginHasLiteral
	rdfs:isDefinedBy <https://github.com/stazh/sw-ehedaten/tree/main/ontology/archiving#>;
	a owl:ObjectProperty;
	rdfs:label "date of origin has literal"@en, "Entstehungszeitraum hat Literal";
	rdfs:comment """Relating a date of origin to its literal."""@en;
	rdfs:domain archiving:Title;
	rdfs:range rdfs:Literal.



#Scope-ID
archiving:recordIsIdentifiedByIdentifier 
	rdfs:isDefinedBy <https://github.com/stazh/sw-ehedaten/tree/main/ontology/archiving#>;
	a rdfs:Class;
	rdfs:label "record is identified by identifier"@en, "Archivverzeichniseinheit wird identifiziert mit Identifikator."@de;
	rdfs:comment """Relating a record to its identifier."""@en;
	rdfs:domain archiving:Record;
	rdfs:range archiving:Identifier.

#Scope-ID
archiving:recordPartIsIdentifiedByIdentifier 
	rdfs:isDefinedBy <https://github.com/stazh/sw-ehedaten/tree/main/ontology/archiving#>;
	a rdfs:Class;
	rdfs:label "record part is identified by identifier"@en, "Archivverzeichniseinheiteil wird identifiziert mit Identifikator."@de;
	rdfs:comment """Relating the record part to its identifier."""@en;
	rdfs:domain archiving:RecordPart;
	rdfs:range archiving:Identifier.

#Signatur
archiving:manifestationIsIdentifiedByIdentifier 
	rdfs:isDefinedBy <https://github.com/stazh/sw-ehedaten/tree/main/ontology/archiving#>;
	a rdfs:Class;
	rdfs:label "manifestation is identified by identifier"@en, "Ausprägung wird identifiziert mit Identifikator."@de;
	rdfs:comment """Relating the manifestation to its identifier."""@en;
	rdfs:domain archiving:manifestation;
	rdfs:range archiving:Identifier.

archiving:identifierHasLiteral
	rdfs:isDefinedBy <https://github.com/stazh/sw-ehedaten/tree/main/ontology/archiving#>;
	a owl:ObjectProperty;
	rdfs:label "identifier has literal"@en, "Identifikator hat Literal";
	rdfs:comment """Relating an identifier to its literal."""@en;
	rdfs:domain archiving:Identifier;
	rdfs:range rdfs:Literal.

archiving:recordIsheldbyArchive
	rdfs:isDefinedBy <https://github.com/stazh/sw-ehedaten/tree/main/ontology/archiving#>;
	a owl:ObjectProperty;
	rdfs:label "record is held by archive"@en, "Archivverzeichniseinheit ist verzeichnet in Archiv";
	rdfs:comment """Relating a record to its archive in which it is recorded and most commonly also in which the manifestation of the record is stored."""@en;
	rdfs:domain archiving:Record;
	rdfs:range archiving:Archive.

archiving:archiveHasNameLiteral
	rdfs:isDefinedBy <https://github.com/stazh/sw-ehedaten/tree/main/ontology/archiving#>;
	a owl:ObjectProperty;
	rdfs:label "archive has name literal"@en, "Archiv hat Namenliteral";
	rdfs:comment """Relating an archive to its name literal."""@en;
	rdfs:domain archiving:Archive;
	rdfs:range rdfs:Literal.


archiving:recordHasProvenance
	rdfs:isDefinedBy <https://github.com/stazh/sw-ehedaten/tree/main/ontology/archiving#>;
	a owl:ObjectProperty;
	rdfs:label "record has provenance"@en, "Archivverzeichniseinheit hat Provenienz";
	rdfs:comment """Relating a record to the agent which holds the role provenance for it. Provenance is the role of an agent (f.e. organization, person), which created the manifestation of the record originally for its own purposes."""@en;
	rdfs:domain archiving:Record;
	rdfs:range archiving:Agent;
	rdfs:subPropertyOf rico:hasProvenance.

archiving:recordPartHasProvenance
	rdfs:isDefinedBy <https://github.com/stazh/sw-ehedaten/tree/main/ontology/archiving#>;
	a owl:ObjectProperty;
	rdfs:label "record part has provenance"@en, "Archivverzeichniseinheitteil hat Provenienz";
	rdfs:comment """Relating a record part to the agent which holds the role provenance for it. Provenance is the role of an agent (f.e. organization, person), which created the manifestation of the record part originally for its own purposes."""@en;
	rdfs:domain archiving:RecordPart;
	rdfs:range archiving:Agent;
	rdfs:subPropertyOf rico:hasProvenance.

archiving:agentHasNameLiteral
	rdfs:isDefinedBy <https://github.com/stazh/sw-ehedaten/tree/main/ontology/archiving#>;
	a owl:ObjectProperty;
	rdfs:label "agent has name literal"@en, "Akteur hat Namenliteral";
	rdfs:comment """Relating an agent to the literal of its name."""@en;
	rdfs:domain archiving:Agent;
	rdfs:range rdfs:Literal.

archiving:referenceHasLiteral
	rdfs:isDefinedBy <https://github.com/stazh/sw-ehedaten/tree/main/ontology/archiving#>;
	a owl:ObjectProperty;
	rdfs:label "reference has name literal"@en, "Referenz hat Literal";
	rdfs:comment """Relating a reference to its literal."""@en;
	rdfs:domain archiving:Reference;
	rdfs:range rdfs:Literal.

archiving:recordHasWebpage
	rdfs:isDefinedBy <https://github.com/stazh/sw-ehedaten/tree/main/ontology/archiving#>;
	a owl:ObjectProperty;
	rdfs:label "record has webpage"@en, "Archivverzeichniseinheit hat Webseite";
	rdfs:comment """Relating a record to the webpage of the entry in an archive information system."""@en;
	rdfs:domain archiving:Record;
	rdfs:range archiving:Webpage.

archiving:recordPartHasWebpage
	rdfs:isDefinedBy <https://github.com/stazh/sw-ehedaten/tree/main/ontology/archiving#>;
	a owl:ObjectProperty;
	rdfs:label "record part has webpage"@en, "Archivverzeichniseinheitteil hat Webseite";
	rdfs:comment """Relating a record part to the webpage of the entry in an archive information system."""@en;
	rdfs:domain archiving:RecordPart;
	rdfs:range archiving:Webpage.

archiving:webpageHasURL
	rdfs:isDefinedBy <https://github.com/stazh/sw-ehedaten/tree/main/ontology/archiving#>;
	a owl:ObjectProperty;
	rdfs:label "webpage has URL"@en, "Webseite hat URL";
	rdfs:comment """Relating a webpage to its URL."""@en;
	rdfs:domain archiving:Webpage;
	rdfs:range xsd:anyURI;
	rdfs:subPropertyOf electronic-information:webpageHasURL.

archiving:recordHasAdditionalContent
	rdfs:isDefinedBy <https://github.com/stazh/sw-ehedaten/tree/main/ontology/archiving#>;
	a owl:ObjectProperty;
	rdfs:label "record has additional content"@en, "Archivverzeichniseinheit hat Zusatzinformation";
	rdfs:comment """Relating a record to the some further information about it, which can be of any kind."""@en;
	rdfs:domain archiving:Record;
	rdfs:range archiving:AdditionalContent.

archiving:recordPartHasAdditionalContent
	rdfs:isDefinedBy <https://github.com/stazh/sw-ehedaten/tree/main/ontology/archiving#>;
	a owl:ObjectProperty;
	rdfs:label "record part has additional content"@en, "Archivverzeichniseinheitteil hat Zusatzinformation";
	rdfs:comment """Relating a record part to the some further information about it, which can be of any kind."""@en;
	rdfs:domain archiving:RecordPart;
	rdfs:range archiving:AdditionalContent.

archiving:additionalContentHasLiteral
	rdfs:isDefinedBy <https://github.com/stazh/sw-ehedaten/tree/main/ontology/archiving#>;
	a owl:ObjectProperty;
	rdfs:label "additional content has name literal"@en, "Zusatzinformation hat Literal";
	rdfs:comment """Relating additional content to its literal."""@en;
	rdfs:domain archiving:AdditionalContent;
	rdfs:range rdfs:Literal.

archiving:isRepresentedByRecord
	rdfs:isDefinedBy <https://github.com/stazh/sw-ehedaten/tree/main/ontology/archiving#>;
	a owl:ObjectProperty;
	rdfs:label "is represented by record"@en, "wird durch Archivverzeichniseinheit dargestellt";
	rdfs:comment """Relating something in the world (an event, a thing...) to the record it is represented by."""@en;
	rdfs:domain rdfs:Resource;
	rdfs:range archiving:Record;
	owl:inverseOf archiving:recordRepresents.

archiving:isRepresentedByRecordPart
	rdfs:isDefinedBy <https://github.com/stazh/sw-ehedaten/tree/main/ontology/archiving#>;
	a owl:ObjectProperty;
	rdfs:label "is represented by record part"@en, "wird durch Archivverzeichniseinheitteil dargestellt";
	rdfs:comment """Relating something in the world (an event, a thing...) to the record part it is represented by."""@en;
	rdfs:domain rdfs:Resource;
	rdfs:range archiving:RecordPart;
	owl:inverseOf archiving:recordPartRepresents.

#und dann repräsentiert es einen Eheeintrag im Kirchgemeindebuch. Das wird dann Klasse in Marriage-Konzept. 

archiving:recordRepresents
	rdfs:isDefinedBy <https://github.com/stazh/sw-ehedaten/tree/main/ontology/archiving#>;
	a owl:ObjectProperty;
	rdfs:label "record represents"@en, "Archivverzeichniseinheit stellt dar"@de;
	rdfs:comment """Relating an record to what (an event, a thing...) it represents."""@en;
	rdfs:domain archiving:Record;
	rdfs:range rdfs:Resource;
	owl:inverseOf archiving:isRepresentedByRecord.

archiving:recordPartRepresents
	rdfs:isDefinedBy <https://github.com/stazh/sw-ehedaten/tree/main/ontology/archiving#>;
	a owl:ObjectProperty;
	rdfs:label "record part represents"@en, "Archivverzeichniseinheitteil stellt dar"@de;
	rdfs:comment """Relating an record part to what (an event, a thing...) it represents."""@en;
	rdfs:domain archiving:RecordPart;
	rdfs:range rdfs:Resource;
	owl:inverseOf archiving:isRepresentedByRecordPart.


