@prefix rdfs: <http://www.w3.org/2000/01/rdf-schema#> .
@prefix owl: <http://www.w3.org/2002/07/owl#> .
@prefix xsd: <http://www.w3.org/2001/XMLSchema#> .
@prefix skos: <http://www.w3.org/2004/02/skos/core#> .
@prefix dct: <http://purl.org/dc/terms/> .
@prefix rico: <https://www.ica.org/standards/RiC/ontology#> .

@base <https://github.com/stazh/sw-ehedaten/tree/main/ontology/archiving.> .
@prefix archiving: <https://github.com/stazh/sw-ehedaten/tree/main/ontology/archiving#> .

<https://github.com/stazh/sw-ehedaten/tree/main/ontology/archiving>
	a owl:Ontology;
	dct:license <http://creativecommons.org/licenses/by/3.0/>;
	dct:title "An ontology about archiving"@en;
	dct:description """Formal description of a record, general subclasses, related classes and properties."""@en;
	dct:creator "Rebekka Plüss, research assistant and software developer, States Archive canton of Zürich"@en;
	dct:contributor "Hans Cools, MD, knowledge engineer, ontologist, software developer, University of Basel, Switzerland"@en;
	dct:publisher "States Archive canton of Zürich"@en;
	owl:versionInfo "2021-10-17"^^xsd:date.



    #Signatur --> Instantiation has Identifier

    #Nachname Mann --> RecordPart has Title
    #Vorname Mann
    #Herkunft Mann
    #Nachname Frau
    #Vorname Frau
    #Herkunft Frau 

    #Zusatzinformationen Mann (Inhalt und Form) --> RecordPart has DescriptiveNote

    #Datum Entstehungszeitraum --> TODO aber klar wie. Record und Record Part hat entstehungszeitraum, entstehungszeitraum = ric-o Date.
    
    #Kirchgemeinde Provenienz --> RecordPart or Record has Provenance

    #Seite im Band, Referenz  (Anmerkungen) --> ????

    #Webseite (zum Eintrag in der Archivdatenbank) --> Record, RecordPart has Webpage

#
# CLASSES
#

archiving:Record
	rdfs:isDefinedBy <https://github.com/stazh/sw-ehedaten/tree/main/ontology/archiving#>;
	a rdfs:Class;
	rdfs:label "record"@en, "Archiveinheit"@de;
	rdfs:comment """A record as an entry in an Archive Information System with metadata, which describe the instantiation of the record."""@en;
	rdfs:subClassOf rico:Record.

archiving:RecordPart
	rdfs:isDefinedBy <https://github.com/stazh/sw-ehedaten/tree/main/ontology/archiving#>;
	a rdfs:Class;
	rdfs:label "record part"@en, "Teil einer Archiveinheit"@de;
	rdfs:comment """A record part as an entry in an Archive Information System with metadata, which describe the instantiation of the record part."""@en;
	rdfs:subClassOf rico:RecordPart.

archiving:Title
	rdfs:isDefinedBy <https://github.com/stazh/sw-ehedaten/tree/main/ontology/archiving#>;
	a rdfs:Class;
	rdfs:label "title"@en, "Titel"@de;
	rdfs:comment """The title of the record or the record part."""@en;
	rdfs:subClassOf rico:Tilte.

archiving:CarrierType
	rdfs:isDefinedBy <https://github.com/stazh/sw-ehedaten/tree/main/ontology/archiving#>;
	a rdfs:Class;
	rdfs:label "Carrier type"@en, "Trägertyp"@de;
	rdfs:comment """The physical or electronical carrier of the instantiation of the record, the archival material type. This can be, f. e. paper, digital image,..."""@en;
	rdfs:subClassOf rico:CarrierType.

#TODO: ansehen in RiC-O xyRelation
archiving:Provenance
	rdfs:isDefinedBy <https://github.com/stazh/sw-ehedaten/tree/main/ontology/archiving#>;
	a rdfs:Class;
	rdfs:label "provenance"@en, "Provenienz"@de;
	rdfs:comment """The agent (f.e. organization, person), which created the record originally for its own purposes."""@en.

archiving:Instantiation
	rdfs:isDefinedBy <https://github.com/stazh/sw-ehedaten/tree/main/ontology/archiving#>;
	a rdfs:Class;
	rdfs:label "instantiation"@en, "Ausprägung"@de;
	rdfs:comment """The archived thing to which the record or the record part refers."""@en;
	rdfs:subClassOf rico:Instantiation.

archiving:Volume
	rdfs:isDefinedBy <https://github.com/stazh/sw-ehedaten/tree/main/ontology/archiving#>;
	a rdfs:Class;
	rdfs:label "volume"@en, "Band"@de;
	rdfs:comment """Volume as type of the carrier resp. the archival material type. It is also a special book: One book of a serie of books. One serie is a set of books which are mostly created for the same purpose by the same provenance."""@en;
	rdfs:subClassOf archiving:CarrierType.

archiving:DescriptiveNote
	rdfs:isDefinedBy <https://github.com/stazh/sw-ehedaten/tree/main/ontology/archiving#>;
	a rdfs:Class;
	rdfs:label "descriptive Note"@en, "Zusatzinformation"@de;
	rdfs:comment """Some information about a record or record part. Can be of any kind."""@en.

#TODO: Retrodigitalisat, Mikrofilm

archiving:Identifier
	rdfs:isDefinedBy <https://github.com/stazh/sw-ehedaten/tree/main/ontology/archiving#>;
	a rdfs:Class;
	rdfs:label "identifier"@en, "Identifikator"@de;
	rdfs:comment """The identifying mark with which a record or an record part or instantiation of it can be clearly identified and referenced. In the context of an archive information system, this is usually the signature."""@en;
	rdfs:subClassOf rico:Identifier.

archiving:Title
	rdfs:isDefinedBy <https://github.com/stazh/sw-ehedaten/tree/main/ontology/archiving#>;
	a rdfs:Class;
	rdfs:label "title"@en, "Titel"@de;
	rdfs:comment """."""@en;
	rdfs:subClassOf rico:Title.

archiving:Date
	rdfs:isDefinedBy <https://github.com/stazh/sw-ehedaten/tree/main/ontology/archiving#>;
	a rdfs:Class;
	rdfs:label "date"@en, "Entstehungszeitraum"@de;
	rdfs:comment """The date when the archived item was originally created."""@en;
	rdfs:subClassOf rico:Date.

archiving:Webpage
	rdfs:isDefinedBy <https://github.com/stazh/sw-ehedaten/tree/main/ontology/archiving#>;
	a rdfs:Class;
	rdfs:label "webpage"@en, "Webseite"@de;
	rdfs:comment """Webpage of the record or record part in an archive information system."""@en.

#TODO in NIE-INE Ontologies anschauen
archiving:Reference
	rdfs:isDefinedBy <https://github.com/stazh/sw-ehedaten/tree/main/ontology/archiving#>;
	a rdfs:Class;
	rdfs:label "reference"@en, "Referenz"@de;
	rdfs:comment """A reference to the instantiation of a record or record part."""@en.

#
# PROPERTIES
#

#TODO: RecordPartHasDate

archiving:recordHasRecordPart
	rdfs:isDefinedBy <https://github.com/stazh/sw-ehedaten/tree/main/ontology/archiving#>;
	a owl:ObjectProperty;
	rdfs:label "record has record part"@en, "Archiveinheit hat Archiveinheitteil";
	rdfs:comment """."""@en;
	rdfs:domain archiving:Record;
	rdfs:range archiving:RecordPart;
	rdfs:subPropertyOf rico:hasOrHadPart.

archiving:recordHasInstantiation
	rdfs:isDefinedBy <https://github.com/stazh/sw-ehedaten/tree/main/ontology/archiving#>;
	a owl:ObjectProperty;
	rdfs:label "record has webpage"@en, "Archiveinheit hat Webseite";
	rdfs:comment """Relating a record to its instantiation."""@en;
	rdfs:domain archiving:Record;
	rdfs:range archiving:Instantiation;
	rdfs:subPropertyOf rico:hasInstantiation.

archiving:recordPartHasInstantiation
	rdfs:isDefinedBy <https://github.com/stazh/sw-ehedaten/tree/main/ontology/archiving#>;
	a owl:ObjectProperty;
	rdfs:label "record part has webpage"@en, "Archiveinheitteil hat Webseite";
	rdfs:comment """Relating a record part to its instantiation."""@en;
	rdfs:domain archiving:RecordPart;
	rdfs:range archiving:Instantiation;
	rdfs:subPropertyOf rico:hasInstantiation.

archiving:instantiationHasCarrierType
	rdfs:isDefinedBy <https://github.com/stazh/sw-ehedaten/tree/main/ontology/archiving#>;
	a owl:ObjectProperty;
	rdfs:label "instantiation has carrier type"@en, "Ausprägung hat Trägertyp";
	rdfs:comment """Relating a archive record to its physical or electronical carrier."""@en;
	rdfs:domain archiving:Instantiation;
	rdfs:range archiving:CarrierType;
	rdfs:subPropertyOf rico:hasCarrierType.

#so wie in RiC-O. Besser titel auch als Klasse und dann titel hat literal. Frage geht dann trotzdem Subproperty of? --> Dasselbe bei descriptiveNote

archiving:recordHasTitle
	rdfs:isDefinedBy <https://github.com/stazh/sw-ehedaten/tree/main/ontology/archiving#>;
	a rdfs:Class;
	rdfs:label "record has title"@en, "Archiveinheit hat Titel"@de;
	rdfs:comment """."""@en;
	rdfs:domain archiving:Record;
	rdfs:range archiving:Title;
	rdfs:subPropertyOf rico:hasOrHadTitle.

archiving:recordPartHasTitle
	rdfs:isDefinedBy <https://github.com/stazh/sw-ehedaten/tree/main/ontology/archiving#>;
	a rdfs:Class;
	rdfs:label "record part has title"@en, "Archiveinheitteil hat Titel"@de;
	rdfs:comment """."""@en;
	rdfs:domain archiving:RecordPart;
	rdfs:range archiving:Title;
	rdfs:subPropertyOf rico:hasOrHadTitle. 


#Scope-ID
archiving:recordIsIdentifiedByIdentifier 
	rdfs:isDefinedBy <https://github.com/stazh/sw-ehedaten/tree/main/ontology/archiving#>;
	a rdfs:Class;
	rdfs:label "record is identified by identifier"@en, "Archiveinheit wird identifiziert mit Identifikator."@de;
	rdfs:comment """."""@en;
	rdfs:domain archiving:Record;
	rdfs:range archiving:Identifier.

#Scope-ID
archiving:recordPartIsIdentifiedByIdentifier 
	rdfs:isDefinedBy <https://github.com/stazh/sw-ehedaten/tree/main/ontology/archiving#>;
	a rdfs:Class;
	rdfs:label "record part is identified by identifier"@en, "Archiveinheiteil wird identifiziert mit Identifikator."@de;
	rdfs:comment """."""@en;
	rdfs:domain archiving:RecordPart;
	rdfs:range archiving:Identifier.

#Signatur
archiving:instantiationIsIdentifiedByIdentifier 
	rdfs:isDefinedBy <https://github.com/stazh/sw-ehedaten/tree/main/ontology/archiving#>;
	a rdfs:Class;
	rdfs:label "instantiation is identified by identifier"@en, "Ausprägung wird identifiziert mit Identifikator."@de;
	rdfs:comment """."""@en;
	rdfs:domain archiving:Instantiation;
	rdfs:range archiving:Identifier.

archiving:recordIsheldbyArchive
	rdfs:isDefinedBy <https://github.com/stazh/sw-ehedaten/tree/main/ontology/archiving#>;
	a owl:ObjectProperty;
	rdfs:label "record is held by archive"@en, "Archivdatensatz wird geführt von Archiv";
	rdfs:comment """Relating a record to its archive in which it is stored and recorded. The archive is responsible for the publishing and managing of the record."""@en;
	rdfs:domain archiving:Record;
	rdfs:range archiving:Archive. #TODO

archiving:recordHasProvenance
	rdfs:isDefinedBy <https://github.com/stazh/sw-ehedaten/tree/main/ontology/archiving#>;
	a owl:ObjectProperty;
	rdfs:label "record has provenance"@en, "Archiveinheit hat Provenienz";
	rdfs:comment """Relating a record to the agent, which originally created the record for its own purposes."""@en;
	rdfs:domain archiving:Record;
	rdfs:range archiving:Provenance;
	rdfs:subPropertyOf rico:hasProvenance.

archiving:recordPartHasProvenance
	rdfs:isDefinedBy <https://github.com/stazh/sw-ehedaten/tree/main/ontology/archiving#>;
	a owl:ObjectProperty;
	rdfs:label "record part has provenance"@en, "Archiveinheitteil hat Provenienz";
	rdfs:comment """Relating a record part to the agent, which originally created the record part for its own purposes."""@en;
	rdfs:domain archiving:RecordPart;
	rdfs:range archiving:Provenance;
	rdfs:subPropertyOf rico:hasProvenance.

archiving:recordHasWebpage
	rdfs:isDefinedBy <https://github.com/stazh/sw-ehedaten/tree/main/ontology/archiving#>;
	a owl:ObjectProperty;
	rdfs:label "record has webpage"@en, "Archiveinheit hat Webseite";
	rdfs:comment """Relating a record to the webpage of the entry in an archive information system."""@en;
	rdfs:domain archiving:Record;
	rdfs:range archiving:Webpage.

archiving:recordPartHasWebpage
	rdfs:isDefinedBy <https://github.com/stazh/sw-ehedaten/tree/main/ontology/archiving#>;
	a owl:ObjectProperty;
	rdfs:label "record part has webpage"@en, "Archiveinheitteil hat Webseite";
	rdfs:comment """Relating a record part to the webpage of the entry in an archive information system."""@en;
	rdfs:domain archiving:RecordPart;
	rdfs:range archiving:Webpage.

archiving:recordHasDescriptiveNote
	rdfs:isDefinedBy <https://github.com/stazh/sw-ehedaten/tree/main/ontology/archiving#>;
	a owl:ObjectProperty;
	rdfs:label "record has descriptive note"@en, "Archiveinheit hat Zusatzinformation";
	rdfs:comment """Relating a record to the some further information about it, which can be of any kind."""@en;
	rdfs:domain archiving:Record;
	rdfs:range archiving:DescriptiveNote;
	rdfs:subPropertyOf rico:descriptiveNote.

archiving:recordHPartHasDescriptiveNote
	rdfs:isDefinedBy <https://github.com/stazh/sw-ehedaten/tree/main/ontology/archiving#>;
	a owl:ObjectProperty;
	rdfs:label "record part has descriptive note"@en, "Archiveinheitteil hat Zusatzinformation";
	rdfs:comment """Relating a record part to the some further information about it, which can be of any kind."""@en;
	rdfs:domain archiving:RecordPart;
	rdfs:range archiving:DescriptiveNote;
	rdfs:subPropertyOf rico:descriptiveNote.

archiving:isRepresentedByRecord
	rdfs:isDefinedBy <https://github.com/stazh/sw-ehedaten/tree/main/ontology/archiving#>;
	a owl:ObjectProperty;
	rdfs:label "is represented by record"@en, "wird durch Archiveinheit dargestellt";
	rdfs:comment """Relating something in the world (an event, a thing...) to the record it is represented by."""@en;
	rdfs:domain rdfs:Resource;
	rdfs:range archiving:Record;
	owl:inverseOf archiving:recordRepresents.


#und dann repräsentiert es einen Eheeintrag im Kirchgemeindebuch. Das wird dann Klasse in Marriage-Konzept. 

#Frage: Wie modelliere ich ein Attribut der Beziehung, wie beispielsweise Record Part ist Teil von record mit Referenz....
archiving:recordRepresents
	rdfs:isDefinedBy <https://github.com/stazh/sw-ehedaten/tree/main/ontology/archiving#>;
	a owl:ObjectProperty;
	rdfs:label "record represents"@en, "Archiveinheit stellt dar"@de;
	rdfs:comment """Relating an record to what (an event, a thing...) it represents."""@en;
	rdfs:domain archiving:Record;
	rdfs:range rdfs:Resource;
	owl:inverseOf archiving:isRepresentedByRecord.


#TODO Klassen wie Title, DescriptiveNote hasLiteral...und Webpage hasURL.

