@prefix rdfs: <http://www.w3.org/2000/01/rdf-schema#> .
@prefix owl: <http://www.w3.org/2002/07/owl#> .
@prefix xsd: <http://www.w3.org/2001/XMLSchema#> .
@prefix skos: <http://www.w3.org/2004/02/skos/core#> .
@prefix dct: <http://purl.org/dc/terms/> .
@prefix rico: <https://www.ica.org/standards/RiC/ontology#> .
@prefix nie-ine-information-carrier: <https://e-editiones.ch/ontology/information-carrier#> .
@prefix nie-ine-organization: <https://e-editiones.ch/ontology/organization#> .
@prefix nie-ine-document: <https://e-editiones.ch/ontology/document#> .
@prefix nie-ine-agent: <https://e-editiones.ch/ontology/agent#> .
@prefix nie-ine-electronic-information: <https://e-editiones.ch/ontology/electronic-information#> .

@base <https://github.com/stazh/sw-ehedaten/tree/main/ontology/archiving> .
@prefix archiving: <https://github.com/stazh/sw-ehedaten/tree/main/ontology/archiving#> .

<https://github.com/stazh/sw-ehedaten/tree/main/ontology/archiving>
	a owl:Ontology;
	dct:license <http://creativecommons.org/licenses/by/3.0/>;
	dct:title "An ontology about archiving"@en;
	dct:description """Formal description of a record, general subclasses, related classes and properties."""@en;
	dct:creator "Rebekka Plüss, research assistant and software developer, States Archive canton of Zürich"@en;
	dct:contributor "Hans Cools, MD, knowledge engineer, ontologist, software developer, University of Basel, Switzerland"@en;
	dct:publisher "States Archive canton of Zürich"@en;
	owl:versionInfo "2021-11-05"^^xsd:date.


#
# CLASSES
#
archiving:Archive
	rdfs:isDefinedBy <https://github.com/stazh/sw-ehedaten/tree/main/ontology/archiving#>;
	a rdfs:Class;
	rdfs:label "archive"@en, "Archiv"@de;
	rdfs:comment """Organization having a role of systematic collection, preservation, care and making accessible documents, objects etc. which hold information of the past. There are state archives which document the activities of the administration of the state, or there are archives that collect documents on specific topics - f.e. Social Archive or Women's Archive."""@en;
	rdfs:subClassOf nie-ine-organization:Archive.

archiving:Agent
	rdfs:isDefinedBy <https://github.com/stazh/sw-ehedaten/tree/main/ontology/archiving#>;
	a rdfs:Class;
	rdfs:label "agent"@en, "Akteur"@de;
	rdfs:comment """Something, someone, ... performing in an action."""@en;
	rdfs:subClassOf nie-ine-agent:Agent, rico:Agent.

archiving:Record
	rdfs:isDefinedBy <https://github.com/stazh/sw-ehedaten/tree/main/ontology/archiving#>;
	a rdfs:Class;
	rdfs:label "record"@en, "Archivverzeichniseinheit"@de;
	rdfs:comment """A record as an entry in an Archive Information System with metadata, which describe physical archived things. A record is abstract."""@en;
	rdfs:subClassOf rico:Record.

archiving:RecordPart
	rdfs:isDefinedBy <https://github.com/stazh/sw-ehedaten/tree/main/ontology/archiving#>;
	a rdfs:Class;
	rdfs:label "record part"@en, "Archivverzeichniseinheit-Teil"@de;
	rdfs:comment """A record part as an entry in an Archive Information System with metadata, which describe parts of physicals archived things. A record part is abstract."""@en;
	rdfs:subClassOf rico:RecordPart.

archiving:Title
	rdfs:isDefinedBy <https://github.com/stazh/sw-ehedaten/tree/main/ontology/archiving#>;
	a rdfs:Class;
	rdfs:label "title"@en, "Titel"@de;
	rdfs:comment """The title of the record or the record part."""@en;
	rdfs:subClassOf rico:Title.

archiving:Manifestation
	rdfs:isDefinedBy <https://github.com/stazh/sw-ehedaten/tree/main/ontology/archiving#>;
	a rdfs:Class;
	rdfs:label "manifestation"@en, "Ausprägung"@de;
	rdfs:comment """Carrier of information created by an agent with role provencance. The physical archived thing to which the record or the record part refers. A record or record part can refer to no manifestation, because it is lost or a record or record part can refer to more than one manifestation (f.e. if there exists a digital representation)."""@en;
	rdfs:subClassOf rico:Instantiation, nie-ine-information-carrier:Carrier.

archiving:Volume
	rdfs:isDefinedBy <https://github.com/stazh/sw-ehedaten/tree/main/ontology/archiving#>;
	a rdfs:Class;
	rdfs:label "volume"@en, "Band"@de;
	rdfs:comment """Volume as type of the carrier resp. the archival material type. It is also a special book: One book of a serie of books. One serie is a set of books which are mostly created for the same purpose by the same agent."""@en;
	rdfs:subClassOf archiving:Manifestation, nie-ine-information-carrier:Volume.

archiving:DigitalCopy
	rdfs:isDefinedBy <https://github.com/stazh/sw-ehedaten/tree/main/ontology/archiving#>;
	a rdfs:Class;
	rdfs:label "digital copy"@en, "Digitalisat"@de;
	rdfs:comment """Digital copy as type of the carrier resp. the archival material type."""@en;
	rdfs:subClassOf archiving:Manifestation.

archiving:AdditionalContent
	rdfs:isDefinedBy <https://github.com/stazh/sw-ehedaten/tree/main/ontology/archiving#>;
	a rdfs:Class;
	rdfs:label "additional content"@en, "Zusatzinformation"@de;
	rdfs:comment """Some further information about a record or record part. Can be of any kind."""@en.


archiving:Identifier
	rdfs:isDefinedBy <https://github.com/stazh/sw-ehedaten/tree/main/ontology/archiving#>;
	a rdfs:Class;
	rdfs:label "identifier"@en, "Identifikator"@de;
	rdfs:comment """The identifying mark with which a record or an record part or manifestation of it can be clearly identified and referenced. In the context of an archive information system, this is usually the signature."""@en;
	rdfs:subClassOf rico:Identifier.

archiving:DateOfOrigin
	rdfs:isDefinedBy <https://github.com/stazh/sw-ehedaten/tree/main/ontology/archiving#>;
	a rdfs:Class;
	rdfs:label "date of origin"@en, "Entstehungszeitraum"@de;
	rdfs:comment """The date when the archived thing was originally created."""@en;
	rdfs:subClassOf rico:Date.

archiving:Webpage
	rdfs:isDefinedBy <https://github.com/stazh/sw-ehedaten/tree/main/ontology/archiving#>;
	a rdfs:Class;
	rdfs:label "webpage"@en, "Webseite"@de;
	rdfs:comment """Webpage of the record or record part in an archive information system."""@en;
	rdfs:subClassOf nie-ine-electronic-information:Webpage.

archiving:Reference
	rdfs:isDefinedBy <https://github.com/stazh/sw-ehedaten/tree/main/ontology/archiving#>;
	a rdfs:Class;
	rdfs:label "reference"@en, "Referenz"@de;
	rdfs:comment """A reference as the information, how a record refers to an other record or record part or vice versa. Same holds for manifestation."""@en.


#
# PROPERTIES
#
archiving:agentHasNameLiteral
	rdfs:isDefinedBy <https://github.com/stazh/sw-ehedaten/tree/main/ontology/archiving#>;
	a owl:DatatypeProperty;
	rdfs:label "agent has name literal"@en, "Akteur hat Namenliteral"@de;
	rdfs:comment """Relating an agent to its name literal"""@en;
	rdfs:domain archiving:Agent;
	rdfs:range rdfs:Literal.

archiving:recordHasRecordPart
	rdfs:isDefinedBy <https://github.com/stazh/sw-ehedaten/tree/main/ontology/archiving#>;
	a owl:ObjectProperty;
	rdfs:label "record has record part"@en, "Archivverzeichniseinheit hat Archivverzeichniseinheit-Teil";
	rdfs:comment """Relating a record part to the record of which it is part of."""@en;
	rdfs:domain archiving:Record;
	rdfs:range archiving:RecordPart;
	rdfs:subPropertyOf rico:hasOrHadPart.

archiving:recordHasReferenceToRecordPart
	rdfs:isDefinedBy <https://github.com/stazh/sw-ehedaten/tree/main/ontology/archiving#>;
	a owl:ObjectProperty;
	rdfs:label "record has reference to record part"@en, "Archivverzeichniseinheit hat Referenz zu Archivverzeichniseinheit-Teil";
	rdfs:comment """Relating a record part to the record of which it is part of and at the same time it is said that a reference to this relation exists."""@en;
	rdfs:domain archiving:Record;
	rdfs:range archiving:RecordPart;
	rdfs:subPropertyOf rico:hasOrHadPart.

archiving:recordHasManifestation
	rdfs:isDefinedBy <https://github.com/stazh/sw-ehedaten/tree/main/ontology/archiving#>;
	a owl:ObjectProperty;
	rdfs:label "record has manifestation"@en, "Archivverzeichniseinheit hat Ausprägung";
	rdfs:comment """Relating a record to its manifestation."""@en;
	rdfs:domain archiving:Record;
	rdfs:range archiving:Manifestation;
	rdfs:subPropertyOf rico:hasInstantiation.

archiving:recordPartHasManifestation
	rdfs:isDefinedBy <https://github.com/stazh/sw-ehedaten/tree/main/ontology/archiving#>;
	a owl:ObjectProperty;
	rdfs:label "record part has manifestation"@en, "Archivverzeichniseinheit-Teil hat Ausprägung";
	rdfs:comment """Relating a record part to its manifestation."""@en;
	rdfs:domain archiving:RecordPart;
	rdfs:range archiving:Manifestation;
	rdfs:subPropertyOf rico:hasInstantiation.

archiving:recordHasTitle
	rdfs:isDefinedBy <https://github.com/stazh/sw-ehedaten/tree/main/ontology/archiving#>;
	a owl:ObjectProperty;
	rdfs:label "record has title"@en, "Archivverzeichniseinheit hat Titel"@de;
	rdfs:comment """Relating a record to its title."""@en;
	rdfs:domain archiving:Record;
	rdfs:range archiving:Title;
	rdfs:subPropertyOf rico:hasOrHadTitle.

archiving:recordHasTitleLiteral
	rdfs:isDefinedBy <https://github.com/stazh/sw-ehedaten/tree/main/ontology/archiving#>;
	a owl:DatatypeProperty;
	rdfs:label "record has title literal"@en, "Archivverzeichniseinheit hat Titelliteral"@de;
	rdfs:comment """Relating a record to its title literal."""@en;
	rdfs:domain archiving:Record;
	rdfs:range rdfs:Literal;
	rdfs:subPropertyOf rico:title.

archiving:recordPartHasTitle
	rdfs:isDefinedBy <https://github.com/stazh/sw-ehedaten/tree/main/ontology/archiving#>;
	a owl:ObjectProperty;
	rdfs:label "record part has title"@en, "Archivverzeichniseinheit-Teil hat Titel"@de;
	rdfs:comment """Relating a record part to its title."""@en;
	rdfs:domain archiving:RecordPart;
	rdfs:range archiving:Title;
	rdfs:subPropertyOf rico:hasOrHadTitle. 

archiving:recordPartHasTitleLiteral
	rdfs:isDefinedBy <https://github.com/stazh/sw-ehedaten/tree/main/ontology/archiving#>;
	a owl:DatatypeProperty;
	rdfs:label "record part has title literal"@en, "Archivverzeichniseinheit-Teil hat Titelliteral"@de;
	rdfs:comment """Relating a record part to its title literal."""@en;
	rdfs:domain archiving:RecordPart;
	rdfs:range rdfs:Literal;
	rdfs:subPropertyOf rico:title.

archiving:titleHasLiteral
	rdfs:isDefinedBy <https://github.com/stazh/sw-ehedaten/tree/main/ontology/archiving#>;
	a owl:ObjectProperty;
	rdfs:label "title has literal"@en, "Titel hat Literal";
	rdfs:comment """Relating a title to its literal."""@en;
	rdfs:domain archiving:Title;
	rdfs:range rdfs:Literal.

archiving:recordHasDateOfOrigin
	rdfs:isDefinedBy <https://github.com/stazh/sw-ehedaten/tree/main/ontology/archiving#>;
	a owl:ObjectProperty;
	rdfs:label "record has date of origin"@en, "Archivverzeichniseinheit hat Entstehungszeitraum"@de;
	rdfs:comment """Relating a date of origin to a record."""@en;
	rdfs:domain archiving:Record;
	rdfs:range archiving:DateOfOrigin;
	rdfs:subPropertyOf rico:hasBeginningDate.

archiving:recordPartHasDateOfOrigin
	rdfs:isDefinedBy <https://github.com/stazh/sw-ehedaten/tree/main/ontology/archiving#>;
	a owl:ObjectProperty;
	rdfs:label "record part has dat of origin"@en, "Archivverzeichniseinheitteil hat Entstehungszeitraum"@de;
	rdfs:comment """Relating a date of origin to a record part."""@en;
	rdfs:domain archiving:RecordPart;
	rdfs:range archiving:DateOfOrigin;
	rdfs:subPropertyOf rico:hasBeginningDate.

archiving:dateOfOriginHasLiteral
	rdfs:isDefinedBy <https://github.com/stazh/sw-ehedaten/tree/main/ontology/archiving#>;
	a owl:DatatypeProperty;
	rdfs:label "date of origin has literal"@en, "Entstehungszeitraum hat Literal";
	rdfs:comment """Relating a date of origin to its literal."""@en;
	rdfs:domain archiving:Title;
	rdfs:range rdfs:Literal;
	rdfs:subPropertyOf rico:creationDate.

archiving:recordHasdateOfOriginLiteral
	rdfs:isDefinedBy <https://github.com/stazh/sw-ehedaten/tree/main/ontology/archiving#>;
	a owl:DatatypeProperty;
	rdfs:label "record has date of origin literal"@en, "Archivverzeichniseinheit hat Entstehungszeitraum-Literal";
	rdfs:comment """Relating a record to the date of origin literal."""@en;
	rdfs:domain archiving:Record;
	rdfs:range rdfs:Literal;
	rdfs:subPropertyOf rico:creationDate.

archiving:recordPartHasdateOfOriginLiteral
	rdfs:isDefinedBy <https://github.com/stazh/sw-ehedaten/tree/main/ontology/archiving#>;
	a owl:DatatypeProperty;
	rdfs:label "record part has date of origin literal"@en, "Archivverzeichniseinheit-Teil hat Entstehungszeitraum-Literal";
	rdfs:comment """Relating a record part to the date of origin literal."""@en;
	rdfs:domain archiving:RecordPart;
	rdfs:range rdfs:Literal;
	rdfs:subPropertyOf rico:creationDate.

#Scope-ID
archiving:recordIsIdentifiedByIdentifier 
	rdfs:isDefinedBy <https://github.com/stazh/sw-ehedaten/tree/main/ontology/archiving#>;
	a owl:ObjectProperty;
	rdfs:label "record is identified by identifier"@en, "Archivverzeichniseinheit wird identifiziert mit Identifikator."@de;
	rdfs:comment """Relating a record to its identifier."""@en;
	rdfs:domain archiving:Record;
	rdfs:range archiving:Identifier.

archiving:recordIsIdentifiedByIdentifierLiteral
	rdfs:isDefinedBy <https://github.com/stazh/sw-ehedaten/tree/main/ontology/archiving#>;
	a owl:DatatypeProperty;
	rdfs:label "record is identified by identifier literal"@en, "Archivverzeichniseinheit wird identifiziert mit Identifikator-Literal."@de;
	rdfs:comment """Relating a record to its identifier literal."""@en;
	rdfs:domain archiving:Record;
	rdfs:range rdfs:Literal;
	rdfs:subPropertyOf rico:identifier.

#Scope-ID
archiving:recordPartIsIdentifiedByIdentifier 
	rdfs:isDefinedBy <https://github.com/stazh/sw-ehedaten/tree/main/ontology/archiving#>;
	a owl:ObjectProperty;
	rdfs:label "record part is identified by identifier"@en, "Archivverzeichniseinheiteil wird identifiziert mit Identifikator."@de;
	rdfs:comment """Relating the record part to its identifier."""@en;
	rdfs:domain archiving:RecordPart;
	rdfs:range archiving:Identifier.

archiving:recordPartIsIdentifiedByIdentifierLiteral
	rdfs:isDefinedBy <https://github.com/stazh/sw-ehedaten/tree/main/ontology/archiving#>;
	a owl:DatatypeProperty;
	rdfs:label "record part is identified by identifier literal"@en, "Archivverzeichniseinheit-Teil wird identifiziert mit Identifikator-Literal."@de;
	rdfs:comment """Relating a record part to its identifier literal."""@en;
	rdfs:domain archiving:RecordPart;
	rdfs:range rdfs:Literal;
	rdfs:subPropertyOf rico:identifier.

#Signatur
archiving:manifestationIsIdentifiedByIdentifier 
	rdfs:isDefinedBy <https://github.com/stazh/sw-ehedaten/tree/main/ontology/archiving#>;
	a owl:ObjectProperty;
	rdfs:label "manifestation is identified by identifier"@en, "Ausprägung wird identifiziert mit Identifikator."@de;
	rdfs:comment """Relating the manifestation to its identifier."""@en;
	rdfs:domain archiving:Manifestation;
	rdfs:range archiving:Identifier.

archiving:manifestationIsIdentifiedByIdentifierLiteral 
	rdfs:isDefinedBy <https://github.com/stazh/sw-ehedaten/tree/main/ontology/archiving#>;
	a owl:DatatypeProperty;
	rdfs:label "manifestation is identified by identifier literal"@en, "Ausprägung wird identifiziert mit Identifikator-Literal."@de;
	rdfs:comment """Relating the manifestation to its identifier literal."""@en;
	rdfs:domain archiving:Manifestation;
	rdfs:range rdfs:Literal;
	rdfs:subPropertyOf rico:identifier.

archiving:identifierHasLiteral
	rdfs:isDefinedBy <https://github.com/stazh/sw-ehedaten/tree/main/ontology/archiving#>;
	a owl:DatatypeProperty;
	rdfs:label "identifier has literal"@en, "Identifikator hat Literal";
	rdfs:comment """Relating an identifier to its literal."""@en;
	rdfs:domain archiving:Identifier;
	rdfs:range rdfs:Literal.

archiving:recordIsheldbyArchive
	rdfs:isDefinedBy <https://github.com/stazh/sw-ehedaten/tree/main/ontology/archiving#>;
	a owl:ObjectProperty;
	rdfs:label "record is held by archive"@en, "Archivverzeichniseinheit ist verzeichnet in Archiv";
	rdfs:comment """Relating a record to its archive in which it is recorded and most commonly also in which the manifestation of the record is stored."""@en;
	rdfs:domain archiving:Record;
	rdfs:range archiving:Archive.

archiving:archiveHasNameLiteral
	rdfs:isDefinedBy <https://github.com/stazh/sw-ehedaten/tree/main/ontology/archiving#>;
	a owl:DatatypeProperty;
	rdfs:label "archive has name literal"@en, "Archiv hat Namenliteral";
	rdfs:comment """Relating an archive to its name literal."""@en;
	rdfs:domain archiving:Archive;
	rdfs:range rdfs:Literal.

archiving:recordHasProvenance
	rdfs:isDefinedBy <https://github.com/stazh/sw-ehedaten/tree/main/ontology/archiving#>;
	a owl:ObjectProperty;
	rdfs:label "record has provenance"@en, "Archivverzeichniseinheit hat Provenienz";
	rdfs:comment """Relating a record to the agent which holds the role provenance for it. Provenance is the role of an agent (f.e. organization, person), which created the manifestation of the record originally for its own purposes."""@en;
	rdfs:domain archiving:Record;
	rdfs:range archiving:Agent;
	rdfs:subPropertyOf rico:hasProvenance.

archiving:recordHasProvenanceLiteral
	rdfs:isDefinedBy <https://github.com/stazh/sw-ehedaten/tree/main/ontology/archiving#>;
	a owl:DatatypeProperty;
	rdfs:label "record has provenance literal"@en, "Archivverzeichniseinheit hat Provenienz-Literal";
	rdfs:comment """Relating a record to the literal of the agent which holds the role provenance for it. Provenance is the role of an agent (f.e. organization, person), which created the manifestation of the record originally for its own purposes."""@en;
	rdfs:domain archiving:Record;
	rdfs:range rdfs:Literal.

archiving:recordPartHasProvenance
	rdfs:isDefinedBy <https://github.com/stazh/sw-ehedaten/tree/main/ontology/archiving#>;
	a owl:ObjectProperty;
	rdfs:label "record part has provenance"@en, "Archivverzeichniseinheit-Teil hat Provenienz";
	rdfs:comment """Relating a record part to the agent which holds the role provenance for it. Provenance is the role of an agent (f.e. organization, person), which created the manifestation of the record part originally for its own purposes."""@en;
	rdfs:domain archiving:RecordPart;
	rdfs:range archiving:Agent;
	rdfs:subPropertyOf rico:hasProvenance.

archiving:recordPartHasProvenanceLiteral
	rdfs:isDefinedBy <https://github.com/stazh/sw-ehedaten/tree/main/ontology/archiving#>;
	a owl:DatatypeProperty;
	rdfs:label "record part has provenance literal"@en, "Archivverzeichniseinheit-Teil hat Provenienz-Literal";
	rdfs:comment """Relating a record part to the literal of the agent which holds the role provenance for it. Provenance is the role of an agent (f.e. organization, person), which created the manifestation of the record part originally for its own purposes."""@en;
	rdfs:domain archiving:RecordPart;
	rdfs:range rdfs:Literal.

archiving:agentHasNameLiteral
	rdfs:isDefinedBy <https://github.com/stazh/sw-ehedaten/tree/main/ontology/archiving#>;
	a owl:DatatypeProperty;
	rdfs:label "agent has name literal"@en, "Akteur hat Namenliteral";
	rdfs:comment """Relating an agent to the literal of its name."""@en;
	rdfs:domain archiving:Agent;
	rdfs:range rdfs:Literal.

archiving:referenceHasLiteral
	rdfs:isDefinedBy <https://github.com/stazh/sw-ehedaten/tree/main/ontology/archiving#>;
	a owl:DatatypeProperty;
	rdfs:label "reference has literal"@en, "Referenz hat Literal";
	rdfs:comment """Relating a reference to its literal."""@en;
	rdfs:domain archiving:Reference;
	rdfs:range rdfs:Literal.

archiving:recordPartHasReferenceLiteral
	rdfs:isDefinedBy <https://github.com/stazh/sw-ehedaten/tree/main/ontology/archiving#>;
	a owl:DatatypeProperty;
	rdfs:label "record part has reference literal"@en, "Archivverzeichniseinheit-Teil hat Referenz-Literal";
	rdfs:comment """Relating a record part to its reference literal."""@en;
	rdfs:domain archiving:RecordPart;
	rdfs:range rdfs:Literal.

archiving:recordHasWebpage
	rdfs:isDefinedBy <https://github.com/stazh/sw-ehedaten/tree/main/ontology/archiving#>;
	a owl:ObjectProperty;
	rdfs:label "record has webpage"@en, "Archivverzeichniseinheit hat Webseite";
	rdfs:comment """Relating a record to the webpage of the entry in an archive information system."""@en;
	rdfs:domain archiving:Record;
	rdfs:range archiving:Webpage.

archiving:recordHasWebpageURI
	rdfs:isDefinedBy <https://github.com/stazh/sw-ehedaten/tree/main/ontology/archiving#>;
	a owl:DatatypeProperty;
	rdfs:label "record has webpage URI"@en, "Archivverzeichniseinheit hat Webseite-URI";
	rdfs:comment """Relating a record to the webpage uri of the entry in an archive information system."""@en;
	rdfs:domain archiving:Record;
	rdfs:range xsd:anyURI.

archiving:recordPartHasWebpage
	rdfs:isDefinedBy <https://github.com/stazh/sw-ehedaten/tree/main/ontology/archiving#>;
	a owl:ObjectProperty;
	rdfs:label "record part has webpage"@en, "Archivverzeichniseinheitteil hat Webseite";
	rdfs:comment """Relating a record part to the webpage of the entry in an archive information system."""@en;
	rdfs:domain archiving:RecordPart;
	rdfs:range archiving:Webpage.

archiving:recordPartHasWebpageURI
	rdfs:isDefinedBy <https://github.com/stazh/sw-ehedaten/tree/main/ontology/archiving#>;
	a owl:DatatypeProperty;
	rdfs:label "record part has webpage URI"@en, "Archivverzeichniseinheit-Teil hat Webseite-URI";
	rdfs:comment """Relating a record part to the webpage uri of the entry in an archive information system."""@en;
	rdfs:domain archiving:RecordPart;
	rdfs:range xsd:anyURI.

archiving:digitalCopyHasWebpageURI
	rdfs:isDefinedBy <https://github.com/stazh/sw-ehedaten/tree/main/ontology/archiving#>;
	a owl:DatatypeProperty;
	rdfs:label "digital copy has webpage URI"@en, "Digitalisat hat Webseite-URI";
	rdfs:comment """Relating a digital copy to the webpage uri."""@en;
	rdfs:domain archiving:DigitalCopy;
	rdfs:range xsd:anyURI.

archiving:webpageHasURL
	rdfs:isDefinedBy <https://github.com/stazh/sw-ehedaten/tree/main/ontology/archiving#>;
	a owl:DatatypeProperty;
	rdfs:label "webpage has URL"@en, "Webseite hat URL";
	rdfs:comment """Relating a webpage to its URL."""@en;
	rdfs:domain archiving:Webpage;
	rdfs:range xsd:anyURI;
	rdfs:subPropertyOf nie-ine-electronic-information:webpageHasURL.

archiving:recordHasAdditionalContent
	rdfs:isDefinedBy <https://github.com/stazh/sw-ehedaten/tree/main/ontology/archiving#>;
	a owl:ObjectProperty;
	rdfs:label "record has additional content"@en, "Archivverzeichniseinheit hat Zusatzinformation";
	rdfs:comment """Relating a record to the some further information about it, which can be of any kind."""@en;
	rdfs:domain archiving:Record;
	rdfs:range archiving:AdditionalContent.

archiving:recordHasAdditionalContentLiteral
	rdfs:isDefinedBy <https://github.com/stazh/sw-ehedaten/tree/main/ontology/archiving#>;
	a owl:DatatypeProperty;
	rdfs:label "record has additional content literal"@en, "Archivverzeichniseinheit hat Zusatzinformation-Literal";
	rdfs:comment """Relating a record to the literal of some further information about it, which can be of any kind."""@en;
	rdfs:domain archiving:Record;
	rdfs:range rdfs:Literal;
	rdfs:subPropertyOf rico:scopeAndContent.

archiving:recordPartHasAdditionalContent
	rdfs:isDefinedBy <https://github.com/stazh/sw-ehedaten/tree/main/ontology/archiving#>;
	a owl:ObjectProperty;
	rdfs:label "record part has additional content"@en, "Archivverzeichniseinheitteil hat Zusatzinformation";
	rdfs:comment """Relating a record part to the some further information about it, which can be of any kind."""@en;
	rdfs:domain archiving:RecordPart;
	rdfs:range archiving:AdditionalContent.

archiving:recordPartHasAdditionalContentLiteral
	rdfs:isDefinedBy <https://github.com/stazh/sw-ehedaten/tree/main/ontology/archiving#>;
	a owl:DatatypeProperty;
	rdfs:label "record part has additional content literal"@en, "Archivverzeichniseinheit-Teil hat Zusatzinformation-Literal";
	rdfs:comment """Relating a record part to the literal of some further information about it, which can be of any kind."""@en;
	rdfs:domain archiving:RecordPart;
	rdfs:range rdfs:Literal;
	rdfs:subPropertyOf rico:scopeAndContent.

archiving:additionalContentHasLiteral
	rdfs:isDefinedBy <https://github.com/stazh/sw-ehedaten/tree/main/ontology/archiving#>;
	a owl:DatatypeProperty;
	rdfs:label "additional content has name literal"@en, "Zusatzinformation hat Literal";
	rdfs:comment """Relating additional content to its literal."""@en;
	rdfs:domain archiving:AdditionalContent;
	rdfs:range rdfs:Literal.

archiving:isRepresentedByRecord
	rdfs:isDefinedBy <https://github.com/stazh/sw-ehedaten/tree/main/ontology/archiving#>;
	a owl:ObjectProperty;
	rdfs:label "is represented by record"@en, "wird durch Archivverzeichniseinheit dargestellt";
	rdfs:comment """Relating something in the world (an event, a thing...) to the record it is represented by."""@en;
	rdfs:domain rdfs:Resource;
	rdfs:range archiving:Record;
	owl:inverseOf archiving:recordRepresents.

archiving:isRepresentedByRecordPart
	rdfs:isDefinedBy <https://github.com/stazh/sw-ehedaten/tree/main/ontology/archiving#>;
	a owl:ObjectProperty;
	rdfs:label "is represented by record part"@en, "wird durch Archivverzeichniseinheitteil dargestellt";
	rdfs:comment """Relating something in the world (an event, a thing...) to the record part it is represented by."""@en;
	rdfs:domain rdfs:Resource;
	rdfs:range archiving:RecordPart;
	owl:inverseOf archiving:recordPartRepresents.

#und dann repräsentiert es einen Eheeintrag im Kirchgemeindebuch. Das wird dann Klasse in Marriage-Konzept. 

archiving:recordRepresents
	rdfs:isDefinedBy <https://github.com/stazh/sw-ehedaten/tree/main/ontology/archiving#>;
	a owl:ObjectProperty;
	rdfs:label "record represents"@en, "Archivverzeichniseinheit stellt dar"@de;
	rdfs:comment """Relating an record to what (an event, a thing...) it represents."""@en;
	rdfs:domain archiving:Record;
	rdfs:range rdfs:Resource;
	owl:inverseOf archiving:isRepresentedByRecord.

archiving:recordPartRepresents
	rdfs:isDefinedBy <https://github.com/stazh/sw-ehedaten/tree/main/ontology/archiving#>;
	a owl:ObjectProperty;
	rdfs:label "record part represents"@en, "Archivverzeichniseinheitteil stellt dar"@de;
	rdfs:comment """Relating an record part to what (an event, a thing...) it represents."""@en;
	rdfs:domain archiving:RecordPart;
	rdfs:range rdfs:Resource;
	owl:inverseOf archiving:isRepresentedByRecordPart.


